src/Find_tree_stack.thy
@@ -1,45 +1,35 @@
 theory Find_tree_stack imports Prelude Tree_stack "~~/src/HOL/Library/Code_Target_Nat" begin
 
-
 (* the search key is not really needed - it is a parameter of all these defns; the xs and zs are the other leaves not in t *)
-datatype fts_focus_t = Focus core_t
-
+type_synonym fts_focus_t = "Tree core_t"
+  
 type_synonym fts_state_t = "fts_focus_t * tree_stack_t"
 
-definition dest_fts_focus :: "fts_focus_t \<Rightarrow> core_t" where 
-"dest_fts_focus f = (case f of Focus(c) \<Rightarrow> c)"
-
-lemma [simp]: "(Focus c) |> dest_fts_focus = c"
- apply(simp add: rev_apply_def dest_fts_focus_def)
- done
-
 definition tree_to_fts :: "key => Tree => fts_state_t" where
-"tree_to_fts k t = (Focus( mk_core (k,[],None,t,None,[])), [])"
+"tree_to_fts k t = (
+  let f = \<lparr>f_k=k, f_tss1=[], f_kl=None,f_t=t,f_ku=None,f_tss2=[] \<rparr> in
+  (f,[])
+)"
 
 
 (* wellformed_fts ---------------------------------------- *)
 
 definition wellformed_fts_focus :: "key \<Rightarrow> ms_t \<Rightarrow> fts_focus_t => bool" where
-"wellformed_fts_focus k0 ms f = (wellformed_core k0 ms (f|>dest_fts_focus))"
+"wellformed_fts_focus k0 ms f = (
+  let t = f|>f_t in
+  wf_core k0 (t|>tree_to_keys) f &
+  wellformed_tree ms t
+)"
 
-(*begin wf fts1 definition*)
 (* tr: interaction between focus and context *)
 definition wellformed_fts_1 :: "fts_state_t => bool" where
 "wellformed_fts_1 fts = (
-  let (f,ts) = fts in
+  let (c,ts) = fts in
   case ts of
   Nil => True
-  | cn#xs => (    
-    let (c1,c2) = cn in
-    let (k,xs,l,t,u,zs) = f|>dest_fts_focus|>dest_core in
-    let (_,rs,i) = c2|>dest_ksrsi in
-    let b0 = (t = rs!i) in
-    let b2 = (cnode_to_bound cn = (l,u)) in  (* ensure bounds are linked *)
-    b0&b2)
+  | p#xs => (mk_child p = c)
 )"
-(*end wf fts1 definition*)
 
-(*begin wf fts definition*)
 definition wellformed_fts :: "key \<Rightarrow> fts_state_t => bool" where
 "wellformed_fts k0 fts = (
   let (f,ts) = fts in
@@ -47,87 +37,43 @@ definition wellformed_fts :: "key \<Rightarrow> fts_state_t => bool" where
   wellformed_ts k0 ts
   & wellformed_fts_focus k0 ms f
   & wellformed_fts_1 fts)"
-(*end wf fts definition*)
 
 
 
 (* step_fts ---------------------------------------- *)
 
-definition indexes_to_trees :: "Tree list \<Rightarrow> nat list \<Rightarrow> Tree list" where
-"indexes_to_trees rs is = (is |> List.map (% i. rs!i))"
-
-(*
-definition indexes_to_leaves :: "Tree list \<Rightarrow> nat list \<Rightarrow> leaves_t" where
-"indexes_to_leaves rs is = (indexes_to_trees rs is |> List.map tree_to_leaves |> List.concat)"
-*)
-
-definition split_list :: "'a list \<Rightarrow> nat \<Rightarrow> ('a list * 'a * 'a list)" where
-"split_list rs i = (
-  let valid = from_to 0 (length rs -1) in (* valid indexes *)
-  let xs = valid |> filter (% n. n < i) in
-  let zs = valid |> filter (% n. n > i) in
-  (xs|>map (% j. rs!j),
-   rs!i,
-   zs|>map (% j. rs!j))
-)"
-
 (*tr: stops when gets to leaf; no "errors"*)
 (*begin find step definition*)
 definition step_fts :: "fts_state_t => fts_state_t option" where
 "step_fts fts = (
-  let (f,ts) = fts in
-  let (k,xs,l,t,u,zs) = f|>dest_fts_focus|>dest_core in
-  case t of Leaf kvs => None
+  let (f,xs) = fts in
+  case (f|>f_t) of Leaf kvs => None
   | Node(ks,rs) => (
-    let i = search_key_to_index ks k in
-    (* new tree stack ----- *)
-    let cn = (
-      let core = mk_core (k,xs,l,t,u,zs) in
-      let ksrsi = (| cc_ks=ks,cc_rs=rs,cc_i=i |) in
-      (core,ksrsi))
-    in
-    let ts2 = (cn # ts) in
-    (* new focus ----- *)
-    let (tsx,t2,tsy) = split_list rs i in 
-    let (xs',zs') = 
-      (tsx |> List.map tree_to_leaves |> List.concat, tsy |> List.map tree_to_leaves |> List.concat) 
-    in 
-    let (l2,u2) = cnode_to_bound cn in
-    let f2 = Focus( mk_core(k,xs@xs',l2,t2,u2,zs'@zs)) in
-    Some(f2,ts2) ))
-"
-
-
-(* fts_reass ---------------------------------------- *)
-definition fts_reass :: "fts_state_t \<Rightarrow> Tree" where
-"fts_reass fts = (
-  let (f,ts) = fts in
-  let (k,xs,l,t,u,zs) = f|>dest_fts_focus|>dest_core in
-  reass t ts
+    (* new frame - just push the focus.. with ks,rs *)
+    let p = f|>with_t (% _. (ks,rs)) in
+    (* new focus ------ *)
+    let c = mk_child p in
+    Some(c,p#xs) )
 )"
+
+
 
 (* fts_invariant ----------------------------------------- *)
 
 definition fts_trans :: "fts_state_t trans_t" where
 "fts_trans = { (fts,fts'). (step_fts fts = Some fts') }"
 
-(*
-definition fts_invariant :: "(fts_state_t \<Rightarrow> bool) \<Rightarrow> bool" where
-"fts_invariant P = (invariant fts_trans P)"
-*)
 
 (* lemmas ------------------------------------------- *)
 
 (* wf_fts is invariant *)
-(*begin find invariant*)
 definition invariant_wf_fts_lem :: "bool" where
 "invariant_wf_fts_lem = (! k0 P. ((% fts. wellformed_fts k0 fts) = P) \<longrightarrow> invariant fts_trans P)"
-(*end find invariant*)
 
 definition focus_to_leaves :: "fts_focus_t \<Rightarrow> leaves_t" where
 "focus_to_leaves f = (
-  let (k,xs,l,t,u,zs) = f|>dest_fts_focus|>dest_core in
-  xs@(t|>tree_to_leaves)@zs
+  let (k,tss1,l,t,u,tss2) = f|>dest_core in
+  (tss1|>tss_to_leaves)@(t|>tree_to_leaves)@(tss2|>tss_to_leaves)
 )"
 
 (* the focus leaves are invariant *)
